\documentclass{article}
\usepackage{amsmath,amsfonts}
\usepackage[utf8]{inputenc}
\usepackage[T1]{fontenc}
\begin{document}
$$
 \sum_{n=0}^{\infty}{c_n(x-x_0)^n}
$$
$x_0$
$x$
$R > 0$
$|x-x_0|<R$
$|x-x_0|>R$
$x_0$
$I = \{x_0\}$
$R=0$
$x_0 \in \mathbb{R}$
$I = \mathbb{R}$
$R=\infty$
$x_0$
$\displaystyle\sum_{n=0}^{\infty}{c_n(x-x_0)^n}$
$\displaystyle c_n \neq 0$
$\displaystyle \lim_{n\to\infty} \frac{|c_{n+1}|}{|c_n|} = L$
$R$
$\displaystyle R=\frac{1}{L}$
$\displaystyle \frac{1}{\infty} = 0$
$\displaystyle \frac{1}{0} = \infty$
$\displaystyle \sum_{n=0}^{\infty}{c_n(x-x_0)^n}$
$R > 0$
$I$
$f$
$$
\begin{aligned}
    &f: I \to \mathbb{R}\\
    &f(x) = \sum_{n=0}^{\infty}{c_n(x-x_0)^n}
\end{aligned}
$$
$f$
$f$
$]x_0 - R, x_0 + R[$
$$
f'(x) = \sum_{n=1}^{\infty}{n \cdot c_n(x-x_0)^{n-1}}
$$
$f$
$$
\int{f(x)}dx = \sum_{n=0}^{\infty}{\frac{c_n(x-x_0)^{n+1}}{n+1}} + C
$$
$\displaystyle \displaystyle \sum_{n=0}^{\infty}{c_n(x-x_0)^n}$
$x_0 \pm R$
$f$
$x_0 \pm R$
\end{document}
%%Local Variables:
%%TeX-master: t
%%End:
