\documentclass{article}
\usepackage{amsmath,amsfonts}
\usepackage[utf8]{inputenc}
\usepackage[T1]{fontenc}
\begin{document}
$$
\sum_{k=m}^{n}{f(k)}
$$
$k$
$f(k)$
$k$
$m$
$n$
$k$
$k$
$\displaystyle \sum_{k \in K}{c f(x)} = c\sum_{k \in K}{f(x)}$
$\displaystyle \sum_{k \in K}{(f(x) \pm g(x))} = \sum_{k \in K}{f(x)} \pm \sum_{k \in K}{g(x)}$
$\{K_1, K_2\}$
$K$
$\displaystyle \sum_{k \in K}{f(x)} = \sum_{k \in K_1}{f(x)} + \sum_{k \in K_2}{f(x)}$
$p$
$K$
$J \subseteq \mathbb{Z}$
$\sum_{k \in K}{f(p(k))} = \sum_{j \in J}{f(j)}$
$c$
$c$
$$
\sum_{i=1}^{n}{c} = nc
$$
$k$
$$
\sum_{k=1}^{n}{k} = \frac{n(n+1)}{2}
$$
$k$
$X_k$
$$
\sum_{k=1}^{n}{(X_{k+1} - X_k)} = X_{n+1} - X_1
$$
$k$
$$
\sum_{k=1}^{n}{k^2} = \frac{n(n+1)(2n+1)}{6}
$$
\end{document}
%%Local Variables:
%%TeX-master: t
%%End:
